Make mlanguage use angelic&demonic stuff properly

theories/mlanguage/mlanguage.v
@@ -31,8 +31,8 @@ Section mlanguage_mixin.
       head_step p (of_class (ExprVal v), σ) X → False;
     mixin_call_head_step p f vs σ X :
       head_step p (of_class (ExprCall f vs), σ) X ↔
-      (∃ (fn : func) (e2 : expr),
-        p !! f = Some fn ∧ Some e2 = apply_func fn vs ∧ X (e2, σ));
+      (∀ (fn : func) (e2 : expr),
+        p !! f = Some fn → Some e2 = apply_func fn vs → X (e2, σ));
     mixin_call_in_ctx K K' e f vs :
       fill K e = fill K' (of_class (ExprCall f vs)) →
       (∃ K'', K' = comp_ectx K K'') ∨ (∃ v, of_class (ExprVal v) = e);
@@ -155,7 +155,7 @@ Section mlanguage.
   Proof. apply mlanguage_mixin. Qed.
   Lemma call_head_step p f vs σ X :
     head_step p (of_class Λ (ExprCall f vs), σ) X ↔
-    (∃ fn e2, p !! f = Some fn ∧ Some e2 = apply_func fn vs ∧ X (e2, σ)).
+    (∀ fn e2, p !! f = Some fn → Some e2 = apply_func fn vs → X (e2, σ)).
   Proof. apply mlanguage_mixin. Qed.
 
   Lemma fill_empty e : fill empty_ectx e = e.
@@ -210,7 +210,7 @@ Section mlanguage.
   Qed.
   Lemma call_head_step_inv p f vs σ X :
     head_step p (of_class Λ (ExprCall f vs), σ) X →
-    (∃ fn e2, p !! f = Some fn ∧ Some e2 = apply_func fn vs ∧ X (e2, σ)).
+    (∀ fn e2, p !! f = Some fn → Some e2 = apply_func fn vs → X (e2, σ)).
   Proof. eapply call_head_step. Qed.
   Lemma call_head_step_intro p f vs fn σ er :
     p !! f = Some fn →
@@ -218,16 +218,16 @@ Section mlanguage.
     head_step p (of_call Λ f vs, σ) (λ '(e', σ'), e' = er ∧ σ' = σ).
   Proof.
     intros ? ?. eapply call_head_step; intros; simplify_eq.
-    do 2 eexists; repeat split; eauto.
+    split; congruence.
   Qed.
-
+(*
   Definition head_reducible (p : prog Λ) (e : expr Λ) (σ : state Λ) :=
     ∃ X, head_step p (e, σ) X.
   Definition head_irreducible (p : prog Λ) (e : expr Λ) (σ : state Λ) :=
     ∀ X, ¬head_step p (e, σ) X.
   Definition head_stuck (p : prog Λ) (e : expr Λ) (σ : state Λ) :=
     to_val e = None ∧ head_irreducible p e σ.
-
+*)
   (* All non-value redexes are at the root.  In other words, all sub-redexes are
      values. *)
   Definition sub_redexes_are_values (e : expr Λ) :=
@@ -247,14 +247,17 @@ Section mlanguage.
     eapply umrel_upclosed; eauto. intros [? ?]. eauto.
   Qed.
 
-  Definition reducible (p : prog Λ) (e : expr Λ) (σ : state Λ) :=
-    ∃ X, prim_step p (e, σ) X.
+(*
+  Definition reducible_old (p : prog Λ) (e : expr Λ) (σ : state Λ) :=
+    ∃ X, prim_step p (e, σ) X. *)
   Definition irreducible (p : prog Λ) (e : expr Λ) (σ : state Λ) :=
     ∀ X, ¬ prim_step p (e, σ) X.
+  Definition has_ub (p : prog Λ) (e : expr Λ) (σ : state Λ) :=
+    ∃ X, prim_step p (e, σ) X ∧ ∀ x, ¬ X x.
   Definition stuck (p : prog Λ) (e : expr Λ) (σ : state Λ) :=
     to_val e = None ∧ irreducible p e σ.
-  Definition not_stuck (p : prog Λ) (e : expr Λ) (σ : state Λ) :=
-    is_Some (to_val e) ∨ reducible p e σ.
+ (* Definition not_stuck_old (p : prog Λ) (e : expr Λ) (σ : state Λ) :=
+    is_Some (to_val e) ∨ reducible_old p e σ. *)
   Definition reducible_not_ub (p : prog Λ) (e : expr Λ) (σ : state Λ) :=
     ∃ X e' σ', prim_step p (e, σ) X ∧ X (e', σ').
   Definition not_ub (p : prog Λ) (e : expr Λ) (σ : state Λ) :=
@@ -297,37 +300,35 @@ Section mlanguage.
   Qed.
   Lemma of_to_call_flip f vs e : of_call Λ f vs = e → to_call e = Some (f, vs).
   Proof. intros <-. apply to_of_call. Qed.
-
-  Lemma not_reducible p e σ : ¬reducible p e σ ↔ irreducible p e σ.
-  Proof. unfold reducible, irreducible. naive_solver. Qed.
-  Lemma reducible_not_val p e σ : reducible p e σ → to_val e = None.
-  Proof. intros (?&?). eauto using val_stuck. Qed.
+(*
+  Lemma not_reducible_old p e σ : ¬reducible_old p e σ ↔ irreducible p e σ.
+  Proof. unfold reducible_old, irreducible. naive_solver. Qed.
+  Lemma reducible_old_not_val p e σ : reducible_old p e σ → to_val e = None.
+  Proof. intros (?&?). eauto using val_stuck. Qed. *)
   Lemma val_irreducible p e σ : is_Some (to_val e) → irreducible p e σ.
   Proof. intros [??] ??%val_stuck. by destruct (to_val e). Qed.
   Global Instance of_val_inj : Inj (=) (=) (of_val Λ).
   Proof. by intros v v' Hv; apply (inj Some); rewrite -!to_of_val Hv. Qed.
-  Lemma not_not_stuck p e σ : ¬not_stuck p e σ ↔ stuck p e σ.
+  (*
+  Lemma not_not_stuck p e σ : ¬not_stuck_old p e σ ↔ stuck p e σ.
   Proof.
-    rewrite /stuck /not_stuck -not_eq_None_Some -not_reducible.
+    rewrite /stuck /not_stuck_old -not_eq_None_Some -not_reducible_old.
     destruct (decide (to_val e = None)); naive_solver.
-  Qed.
-  Lemma extcall_ctx_irreducible p K f vs σ :
+  Qed. *)
+  Lemma extcall_ctx_has_ub p K f vs σ :
     p !! f = None →
-    irreducible p (fill K (of_class Λ (ExprCall f vs))) σ.
+    has_ub p (fill K (of_class Λ (ExprCall f vs))) σ.
   Proof.
-    intros ? X (K' & e1 & Hfill & Hstep).
-    symmetry in Hfill. pose proof (call_in_ctx_to_val _ _ _ _ _ Hfill) as [[? ->]|[? ?]].
-    - rewrite -fill_comp in Hfill. apply fill_inj in Hfill. subst e1.
-      pose proof (head_ctx_step_val _ _ _ _ _ Hstep) as [->|[? HH]].
-      + rewrite fill_empty in Hstep.
-        apply call_head_step in Hstep as (?&?&?&?&?). congruence.
-      + rewrite /to_val to_of_class // in HH.
-    - apply val_head_stuck in Hstep. congruence.
+    intros H.
+    exists (fun x => False).
+    split; last tauto.
+    econstructor. eexists; split; first done.
+    eapply call_head_step. intros ?? Hc _. rewrite H in Hc; congruence.
   Qed.
 
   Lemma fill_not_val K e : to_val e = None → to_val (fill K e) = None.
   Proof. rewrite !eq_None_not_Some. eauto using fill_val. Qed.
-
+(*
   Lemma not_head_reducible p e σ : ¬head_reducible p e σ ↔ head_irreducible p e σ.
   Proof. unfold head_reducible, head_irreducible. naive_solver. Qed.
 
@@ -349,7 +350,7 @@ Section mlanguage.
     destruct (head_ctx_step_val _ _ _ _ _ Hred') as [HK''|[]%not_eq_None_Some].
     - subst K''. rewrite fill_empty. done.
     - by eapply val_head_stuck.
-  Qed.
+  Qed. *)
 
   Lemma head_prim_step p e1 σ1 X :
     head_step p (e1, σ1) X → prim_step p (e1, σ1) X.
@@ -358,10 +359,10 @@ Section mlanguage.
     - by rewrite fill_empty.
     - intros *. eapply umrel_upclosed; eauto.
       intros [? ?]. rewrite fill_empty //.
-  Qed.
+  Qed. (*
   Lemma head_step_not_stuck p e σ X:
-    head_step p (e, σ) X → not_stuck p e σ.
-  Proof. rewrite /not_stuck /reducible /=. eauto 10 using head_prim_step. Qed.
+    head_step p (e, σ) X → not_stuck_old p e σ.
+  Proof. rewrite /not_stuck_old /reducible_old /=. eauto 10 using head_prim_step. Qed. *)
   Lemma fill_prim_step p K e1 σ1 X X' :
     (∀ e2 σ2, X (e2, σ2) → X' (fill K e2, σ2)) →
     prim_step p (e1, σ1) X →
@@ -381,21 +382,21 @@ Section mlanguage.
     - eapply Hstep.
     - intros ? ? ?. simpl. eexists. eauto.
   Qed.
-
-  Lemma fill_reducible p K e σ : reducible p e σ → reducible p (fill K e) σ.
+(*
+  Lemma fill_reducible_old p K e σ : reducible_old p e σ → reducible_old p (fill K e) σ.
   Proof.
     intros (X & Hstep). exists (λ '(e', σ), ∃ e, e' = fill K e ∧ X (e, σ)).
     eapply fill_prim_step; [| apply Hstep]; eauto.
   Qed.
-  Lemma head_prim_reducible p e σ : head_reducible p e σ → reducible p e σ.
+  Lemma head_prim_reducible_old p e σ : head_reducible p e σ → reducible_old p e σ.
   Proof. intros (X&?). exists X. by apply head_prim_step. Qed.
-  Lemma head_prim_fill_reducible p e K σ :
-    head_reducible p e σ → reducible p (fill K e) σ.
-  Proof. intro. by apply fill_reducible, head_prim_reducible. Qed.
+  Lemma head_prim_fill_reducible_old p e K σ :
+    head_reducible p e σ → reducible_old p (fill K e) σ.
+  Proof. intro. by apply fill_reducible_old, head_prim_reducible_old. Qed.
   Lemma head_prim_irreducible p e σ : irreducible p e σ → head_irreducible p e σ.
   Proof.
-    rewrite -not_reducible -not_head_reducible. eauto using head_prim_reducible.
-  Qed.
+    rewrite -not_reducible_old -not_head_reducible. eauto using head_prim_reducible_old.
+  Qed. *)
 
   Lemma prim_head_step p e σ X :
     prim_step p (e, σ) X → sub_redexes_are_values e → head_step p (e, σ) X.
@@ -404,28 +405,28 @@ Section mlanguage.
     assert (K = empty_ectx) as -> by eauto 10 using val_head_stuck.
     rewrite fill_empty. eapply umrel_upclosed; [apply Hstep|].
     intros [? ?]. rewrite fill_empty //.
-  Qed.
+  Qed. (*
   Lemma prim_head_reducible p e σ :
-    reducible p e σ → sub_redexes_are_values e → head_reducible p e σ.
+    reducible_old p e σ → sub_redexes_are_values e → head_reducible p e σ.
   Proof. intros (X&Hstep) ?. eexists. by eapply prim_head_step. Qed.
   Lemma prim_head_irreducible p e σ :
     head_irreducible p e σ → sub_redexes_are_values e → irreducible p e σ.
   Proof.
-    rewrite -not_reducible -not_head_reducible. eauto using prim_head_reducible.
-  Qed.
+    rewrite -not_reducible_old -not_head_reducible. eauto using prim_head_reducible.
+  Qed. 
 
   Lemma head_stuck_stuck p e σ :
     head_stuck p e σ → sub_redexes_are_values e → stuck p e σ.
   Proof.
     intros [] ?. split; first done. by apply prim_head_irreducible.
-  Qed.
+  Qed. *)
 
-  Lemma head_reducible_prim_step_ctx p K e1 σ1 X :
-    head_reducible p e1 σ1 →
+  Lemma head_reducible_prim_step_ctx p K e1 σ1 X X' :
+    head_step p (e1, σ1) X' →
     prim_step p (fill K e1, σ1) X →
     head_step p (e1, σ1) (λ '(e2', σ2), ∀ e2, e2 = fill K e2' → X (e2, σ2)).
   Proof.
-    intros (X' & HhstepK) (K' & e1' & HKe1 & Hstep).
+    intros HhstepK (K' & e1' & HKe1 & Hstep).
     edestruct (step_by_val p K) as [K'' ?];
       eauto using val_head_stuck; simplify_eq/=.
     rewrite -fill_comp in HKe1; simplify_eq.
@@ -435,17 +436,17 @@ Section mlanguage.
     - apply val_head_stuck in Hstep; simplify_eq.
   Qed.
 
-  Lemma head_reducible_prim_step p e1 σ1 X :
-    head_reducible p e1 σ1 →
+  Lemma head_reducible_prim_step p e1 σ1 X X' :
+    head_step p (e1, σ1) X' →
     prim_step p (e1, σ1) X →
     head_step p (e1, σ1) X.
   Proof.
     intros Hred Hpstep.
-    epose proof (head_reducible_prim_step_ctx _ empty_ectx _ _ X Hred) as Hhstep.
+    epose proof (head_reducible_prim_step_ctx _ empty_ectx _ _ X X' Hred) as Hhstep.
     eapply umrel_upclosed.
     - eapply Hhstep. by rewrite fill_empty.
     - intros [e σ]. rewrite fill_empty. eauto.
-  Qed.
+  Qed. (*
 
   Lemma fill_stuck (P : prog Λ) e σ K : stuck P e σ → stuck P (fill K e) σ.
   Proof.
@@ -459,7 +460,7 @@ Section mlanguage.
       eapply multirelations.umrel_upclosed; eauto. intros [? ?]. rewrite -fill_comp//.
   Qed.
 
-  Lemma fill_not_stuck (P : prog Λ) e σ K : not_stuck P (fill K e) σ → not_stuck P e σ.
+  Lemma fill_not_stuck (P : prog Λ) e σ K : not_stuck_old P (fill K e) σ → not_stuck_old P e σ.
   Proof.
     intros [Hval | Hred].
     - left. by eapply fill_val.
@@ -470,23 +471,23 @@ Section mlanguage.
       rewrite -fill_comp in Heq. apply fill_inj in Heq as ->.
       right. exists (λ '(e, σ), X (fill K e, σ)). do 2 eexists; split_and!; eauto.
       eapply multirelations.umrel_upclosed; eauto. intros [? ?]. rewrite -fill_comp//.
-  Qed.
+  Qed. *)
 
   Lemma prim_step_call_inv p K f vs e' σ X :
     prim_step p (fill K (of_call Λ f vs), σ) X →
-    ∃ er fn,
-      Some er = apply_func fn vs ∧ p !! f = Some fn ∧
+    ∀ er fn,
+      Some er = apply_func fn vs → p !! f = Some fn →
       X (fill K er, σ).
   Proof.
-    intros (K' & e1 & Hctx & Hstep).
+    intros (K' & e1 & Hctx & Hstep) ?? Heq1 Heq2.
     eapply step_by_val in Hstep as H'; eauto; last apply to_val_of_call.
     destruct H' as [K'' Hctx']; subst K'.
     rewrite -fill_comp in Hctx. eapply fill_inj in Hctx.
     destruct (fill_class K'' e1) as [->|Hval].
     - apply is_call_is_class. erewrite of_to_call_flip; eauto.
     - rewrite fill_empty in Hctx. subst e1.
-      eapply call_head_step_inv in Hstep as (?&?&?&?&HX); simplify_eq/=.
-      rewrite -fill_comp fill_empty// in HX. eauto.
+      eapply call_head_step_inv in Hstep. 2-3:done.
+      rewrite -fill_comp fill_empty// in Hstep.
     - apply val_head_stuck in Hstep. apply not_eq_None_Some in Hval. done.
   Qed.
 
@@ -498,10 +499,10 @@ Section mlanguage.
     { rewrite -Heq. rewrite to_of_val. by exists v. }
     eapply val_head_step.
     erewrite <-(of_to_val e1') in Hstep'; eauto.
-  Qed.
+  Qed. (*
 
-  Lemma fill_reducible_prim_step p e σ K X :
-    reducible p e σ →
+  Lemma fill_reducible_old_prim_step p e σ K X :
+    reducible_old p e σ →
     prim_step p (fill K e, σ) X →
     prim_step p (e, σ) (λ '(e2', σ2), ∀ e2, e2 = fill K e2' → X (e2, σ2)).
   Proof.
@@ -513,9 +514,9 @@ Section mlanguage.
     rewrite fill_comp; eauto.
   Qed.
 
-  Lemma reducible_fill p e σ K : reducible p e σ → reducible p (fill K e) σ.
+  Lemma reducible_fill p e σ K : reducible_old p e σ → reducible_old p (fill K e) σ.
   Proof. intros (X & Hstep). eexists. eauto using fill_prim_step'. Qed.
-
+ *)
   Lemma fill_step_inv p K e1' σ1 X :
     to_val e1' = None →
     prim_step p (fill K e1', σ1) X →
@@ -528,10 +529,10 @@ Section mlanguage.
     eapply multirelations.umrel_upclosed; eauto. intros [? ?].
     rewrite -fill_comp//.
   Qed.
-
+(*
   Lemma fill_reducible_inv p K e σ :
-    to_val e = None -> reducible p (fill K e) σ → reducible p e σ.
-  Proof. intros ? (X & Hstep%fill_step_inv); auto. eexists; eauto. Qed.
+    to_val e = None -> reducible_old p (fill K e) σ → reducible_old p e σ.
+  Proof. intros ? (X & Hstep%fill_step_inv); auto. eexists; eauto. Qed. *)
 
   (* Lemma head_call_pure p f vs σ e2 σ' σ2 : *)
   (*   head_step p (of_class Λ (ExprCall f vs), σ) σ e2 σ' → *)
@@ -543,31 +544,31 @@ Section mlanguage.
 
   Lemma call_prim_step_fill p K f vs σ X :
     prim_step p (fill K (of_class Λ (ExprCall f vs)), σ) X →
-    ∃ (fn : func Λ) e2,
-      p !! f = Some fn ∧
-      apply_func fn vs = Some e2 ∧
+    ∀ (fn : func Λ) e2,
+      p !! f = Some fn →
+      apply_func fn vs = Some e2 →
       X (fill K e2, σ).
   Proof.
-    intros (K' & e1 & Hfill%eq_sym & Hstep).
+    intros (K' & e1 & Hfill%eq_sym & Hstep) ?? HH1 HH2.
     pose proof (call_in_ctx _ _ _ _ _ Hfill) as [[K'' ->]|[? Hval]].
     { rewrite -fill_comp in Hfill. apply fill_inj in Hfill. subst e1.
       pose proof (head_ctx_step_val _ _ _ _ _ Hstep) as [->|[? Hval]].
-      { rewrite fill_empty in Hstep. apply call_head_step in Hstep as (fn & ? & ? & ? & ?).
-        eexists _, _; repeat split; eauto. rewrite -!fill_comp fill_empty//. }
+      { rewrite fill_empty in Hstep. eapply call_head_step in Hstep. 2-3:done.
+        rewrite -!fill_comp fill_empty//. }
       { exfalso. rewrite /to_val to_of_class// in Hval. } }
     { exfalso. subst. apply val_head_stuck in Hstep. rewrite /to_val to_of_class// in Hstep. }
   Qed.
 
   Lemma call_prim_step p f vs σ X :
     prim_step p (of_class Λ (ExprCall f vs), σ) X →
-    ∃ (fn : func Λ) e2,
-      p !! f = Some fn ∧
-      apply_func fn vs = Some e2 ∧
+    ∀ (fn : func Λ) e2,
+      p !! f = Some fn →
+      apply_func fn vs = Some e2 →
       X (e2, σ).
   Proof.
-    epose proof (call_prim_step_fill p empty_ectx _ _ _ _) as H.
-    rewrite fill_empty in H. intros (?&?&?&?&HX)%H; subst.
-    eexists _, _. repeat split; eauto. rewrite fill_empty// in HX.
+    intros H. epose proof (call_prim_step_fill p empty_ectx _ _ _ _) as Hp.
+    rewrite !fill_empty in Hp. intros fn e2 H1 H2. specialize (Hp H fn e2 H1).
+    rewrite fill_empty// in Hp. by eapply Hp.
   Qed.
 
   Class IntoVal (e : expr Λ) (v : val) :=
@@ -583,7 +584,7 @@ Section mlanguage.
   Qed.
 
   Record pure_step p (e1 : expr Λ) (e2 : expr Λ) := {
-    pure_step_safe σ1 : reducible p e1 σ1;
+    pure_step_not_val : to_val e1 = None;
     pure_step_det σ1 X :
       prim_step p (e1, σ1) X → X (e2, σ1)
   }.
@@ -595,10 +596,10 @@ Section mlanguage.
     PureExec φ n p e1 e2 →
     PureExec φ n p (fill K e1) (fill K e2).
   Proof.
-    intros H Hφ. specialize (H Hφ). induction H as [|n x y z [Hred Hdet] Hstep IH]; econstructor.
+    intros H Hφ. specialize (H Hφ). induction H as [|n x y z [Hval Hdet] Hstep IH]; econstructor.
     - econstructor.
-      + intros σ1. destruct (Hred σ1) as (?&H). eexists. eapply fill_prim_step'; eauto.
-      + intros σ1 X HH%fill_reducible_prim_step; last apply Hred.
+      + by eapply fill_not_val.
+      + intros σ1 X HH%fill_step_inv; last apply Hval.
         apply Hdet in HH; eauto.
     - apply IH.
   Qed.
@@ -608,9 +609,8 @@ Section mlanguage.
     pure_step p (fill K e1) (fill K e2).
   Proof.
     intros [Hred Hstep]. split.
-    - unfold reducible in *. naive_solver eauto using fill_prim_step'.
-    - intros σ1 X HstepK. specialize (Hred σ1). specialize (Hstep σ1).
-      apply fill_reducible_prim_step in HstepK; auto.
+    - by eapply fill_not_val.
+    - intros σ1 X HstepK%fill_step_inv; last done.
       apply Hstep in HstepK. eauto.
   Qed.
 
@@ -623,7 +623,7 @@ Section mlanguage.
     PureExec P n p e1 e2 →
     PureExec P n p (fill K e1) (fill K e2).
   Proof. rewrite /PureExec; eauto using pure_step_nsteps_ctx. Qed.
-
+(*
   Record pure_head_step p (e1 : expr Λ) (e2 : expr Λ) := {
     pure_head_step_safe σ1 : head_reducible p e1 σ1;
     pure_head_step_det σ1 X :
@@ -639,7 +639,7 @@ Section mlanguage.
     - intros σ X Hstep.
       eapply head_reducible_prim_step, Hp2 in Hstep; eauto.
   Qed.
-
+*)
 End mlanguage.
 
 (* discrete OFE instance for expr *)
